ITree.lean
@@ -1,1 +1,4 @@
-import ITree.Basic
+import ITree.Definition
+import ITree.Effect
+import ITree.Effects
+import ITree.Exec
