ITree/Effects/Conc.lean
@@ -1,0 +1,68 @@
+import ITree.Effect
+import ITree.Definition
+import ITree.Exec
+
+namespace ITree.Effects
+open Lean.Order ITree.Exec
+
+inductive ForkResult : Type u
+| parent | child
+
+inductive concE.I : Type u where
+| fork | kill | yield
+
+def concE : Effect.{u} where
+  I := concE.I
+  O
+  | .fork => ForkResult
+  | .kill => PEmpty
+  | .yield => PUnit
+
+def ConcE.kill {E} [concE -< E] : ITree E α :=
+  .trigger concE (.kill) >>= nofun
+export ConcE (kill)
+
+def ConcE.fork {E} [concE -< E] (child : ITree E PUnit) : ITree E PUnit :=
+  .trigger concE (.fork) >>= λ
+    | .child => child >>= λ _ => kill
+    | .parent => return ⟨⟩
+export ConcE (fork)
+
+@[partial_fixpoint_monotone]
+theorem fork_mono [concE -< E] α [PartialOrder α] (f : α → ITree E PUnit) :
+  monotone f →
+  monotone (λ x => fork (f x)) := by
+  intro hf
+  apply monotone_bind
+  · apply monotone_const
+  · sorry
+
+def ConcE.yield {E} [concE -< E] : ITree E PUnit :=
+  .trigger concE (.yield)
+export ConcE (yield)
+
+def ConcE.yieldAfter [concE -< E] (t : ITree E R) := do
+  let v ← t; yield; return v
+export ConcE (yieldAfter)
+
+@[partial_fixpoint_monotone]
+theorem yieldAfter_mono [concE -< E] α [PartialOrder α] (f : α → ITree E R) :
+  monotone f →
+  monotone (λ x => yieldAfter (f x)) := by
+  intro hf
+  apply monotone_bind
+  · apply hf
+  · apply monotone_const
+
+instance concEH : EHandler concE GE GR (Nat × List (Option (ITree GE GR))) where
+  handle i s k p :=
+    match i with
+    | .fork => p (k .parent) (s.1, s.2 ++ [some (k .child)])
+    | .yield =>
+      let tp' := s.2.set s.1 (some (k ⟨⟩))
+      ∃ i' t', tp'[i']? = some (some t') ∧ p t' (i', tp'.set i' none)
+    | .kill =>
+      ∃ i' t', s.2[i']? = some (some t') ∧ p t' (i', s.2.set i' none)
+  handle_mono := by
+    intros i s k p q himp h; cases i
+    all_goals simp at *; grind
