ITree/Effects/Demonic.lean
@@ -1,0 +1,28 @@
+import ITree.Effect
+import ITree.Definition
+import ITree.Exec
+
+namespace ITree.Effects
+open ITree.Exec
+
+def demonicE (α : Type u) : Effect.{u} where
+  I := α → Prop
+  O p := {a // p a}
+
+def DemonicE.choose {α : Type u} {E : Effect.{u}} [demonicE α -< E] (p : α → Prop) : ITree E {a // p a} :=
+  .trigger (demonicE α) p
+export DemonicE (choose)
+
+def demonicEH (α : Type _) : SEHandler (demonicE α) PUnit where
+  handle i s p := ∃ x, ∃ (h : i x), p ⟨_, h⟩ s
+  handle_mono := by grind
+
+theorem exec_choose {α : Type u} {GE : Effect.{u}} GR σ p q s
+    {k : {x : α // q x} → ITree GE GR}
+    [demonicE α -< GE] (eh : EHandler GE GE GR σ) [hin : InEH (demonicEH α).toEHandler eh]
+    : (∃ (x : α) (h : q x), exec eh (k ⟨x, h⟩) s p) →
+      exec eh (choose q >>= k) s p := by
+  rintro he; unfold choose
+  apply exec.dup
+  apply exec.trigger (demonicEH α).toEHandler
+  simp_all [demonicEH]
