ITree/Effects/Fail.lean
@@ -1,0 +1,18 @@
+import ITree.Effect
+import ITree.Definition
+import ITree.Exec
+
+namespace ITree.Effects
+open ITree.Exec
+
+def failE : Effect.{u} where
+  I := ULift String
+  O _ := PEmpty
+
+def FailE.fail {α : Type u} {E} [failE -< E] (s : String) : ITree.{u} E α :=
+  .trigger (failE) (ULift.up s) >>= nofun
+export FailE (fail)
+
+def failEH : SEHandler failE PUnit where
+  handle i s p := True
+  handle_mono := by grind
