ITree/Effects/Heap.lean
@@ -1,0 +1,53 @@
+import ITree.Effect
+import ITree.Definition
+import ITree.Effects.Demonic
+import ITree.Effects.Fail
+import ITree.Effects.State
+import Std.Data.ExtTreeMap
+
+namespace ITree.Effects
+
+
+protected abbrev heapE.T (Loc : Type u) [Ord Loc] (Val : Type u) :=
+  Std.ExtTreeMap Loc (Option Val)
+abbrev heapE (Loc : Type u) [Ord Loc] (Val : Type u) :=
+  stateE (heapE.T Loc Val)
+abbrev heapEH (Loc : Type u) [Ord Loc] (Val : Type u) :=
+  stateEH (heapE.T Loc Val)
+
+variable {E : Effect.{u}} {Loc : Type u} [Ord Loc] [Std.TransOrd Loc] {Val : Type u}
+
+
+def HeapE.storeOpt [heapE Loc Val -< E] (l : Loc) (v : Option Val) : ITree E (Option Val) := do
+  let hmap ← get
+  set (hmap.insert l v)
+  return hmap[l]?.join
+export HeapE (storeOpt)
+
+def HeapE.store? [heapE Loc Val -< E] (l : Loc) (v : Val) : ITree E (Option Val) :=
+  storeOpt l (some v)
+export HeapE (store?)
+
+def HeapE.store! [heapE Loc Val -< E] [failE -< E] (l : Loc) (v : Val) : ITree E Val := do
+  let some v ← store? l v
+    | fail "Storing in unallocated memory"
+  return v
+export HeapE (store!)
+
+def HeapE.load? [heapE Loc Val -< E] (l : Loc) : ITree E (Option Val) := do
+  let hmap ← get
+  return hmap[l]?.join
+export HeapE (load?)
+
+def HeapE.load! [heapE Loc Val -< E] [failE -< E] (l : Loc) : ITree E Val := do
+  let some v ← load? l
+    | fail "Loading from unallocated memory"
+  return v
+export HeapE (load!)
+
+def HeapE.alloc [heapE Loc Val -< E] [demonicE Loc -< E] (v : Val) : ITree E Loc := do
+  let hmap ← get
+  let ⟨l, _⟩ ← choose (λ l => l ∉ hmap)
+  set (hmap.insert l v)
+  return l
+export HeapE (alloc)
