ITree/Effects/State.lean
@@ -1,0 +1,64 @@
+import ITree.Effect
+import ITree.Definition
+import ITree.Exec
+
+namespace ITree.Effects
+open ITree.Exec
+
+def stateE (α : Type u) : Effect.{u} where
+  I := (α → α)
+  O _ := α
+
+def StateE.modify {α : Type u} {E} [stateE α -< E] (f : α → α) : ITree E α :=
+  .trigger (stateE α) f
+
+def StateE.get {α : Type u} {E} [stateE α -< E] : ITree E α :=
+  modify id
+
+def StateE.set {α : Type u} {E} [stateE α -< E] (a : α) : ITree E PUnit :=
+  modify (λ _ => a) >>= λ _ => return ⟨⟩
+
+def StateE.modifyGet {α : Type u} {β} {E} [stateE α -< E] (f : α → Prod β α) : ITree E β :=
+  do let (x, s) := f (← StateE.get); StateE.set s; return x
+
+set_option synthInstance.checkSynthOrder false in
+instance [stateE α -< E] : MonadStateOf α (ITree E) where
+  get := StateE.get
+  set := StateE.set
+  modifyGet := StateE.modifyGet
+
+def stateEH (α : Type u) : SEHandler (stateE α) α where
+  handle i s p := p s (i s)
+  handle_mono := by grind
+
+theorem exec_stateE_get {α : Type u} {GE : Effect.{u}} GR σ p s
+    {k : α → ITree GE GR}
+    [stateE α -< GE] (eh : EHandler GE GE GR σ) [hin : InEH (stateEH α).toEHandler eh]
+    : exec eh (k (hin.getState s)) s p →
+      exec eh (StateE.get >>= k) s p := by
+  rintro he; simp [StateE.get]
+  apply exec.dup
+  apply exec.trigger (stateEH _).toEHandler
+  simp_all [stateEH]
+
+theorem exec_get {α : Type u} {GE : Effect.{u}} GR σ p s
+    {k : α → ITree GE GR}
+    [stateE α -< GE] (eh : EHandler GE GE GR σ) [hin : InEH (stateEH α).toEHandler eh]
+    : exec eh (k (hin.getState s)) s p →
+      exec eh (get >>= k) s p := exec_stateE_get GR σ p s eh
+
+theorem exec_stateE_set {α : Type u} {GE : Effect.{u}} GR σ p s (s' : α)
+    {k : PUnit → ITree GE GR}
+    [stateE α -< GE] (eh : EHandler GE GE GR σ) [hin : InEH (stateEH α).toEHandler eh]
+    : exec eh (k ⟨⟩) (hin.putState s' s) p →
+      exec eh (StateE.set s' >>= k) s p := by
+  rintro he; simp [StateE.set]
+  apply exec.dup
+  apply exec.trigger (stateEH _).toEHandler
+  simp_all [stateEH]
+
+theorem exec_set {α : Type u} {GE : Effect.{u}} GR σ p s (s' : α)
+    {k : PUnit → ITree GE GR}
+    [stateE α -< GE] (eh : EHandler GE GE GR σ) [hin : InEH (stateEH α).toEHandler eh]
+    : exec eh (k ⟨⟩) (hin.putState s' s) p →
+      exec eh (set s' >>= k) s p := exec_stateE_set GR σ p s s' eh
