Test/ITree.lean
@@ -1,0 +1,20 @@
+import ITree
+
+namespace Test
+open ITree
+
+def f {E R} : ITree E R := f
+partial_fixpoint
+
+def spin2 {E R} : ITree E R := ITree.tau spin2
+partial_fixpoint
+
+example {E R} : @spin2 E R = spin2 := by unfold spin2; rfl
+
+-- TODO: I did not expect this to work. I guess it works, but we cannot prove it monotone
+def test (t1 : ITree E R) : ITree E R :=
+  match t1.unfold with
+  | .ret r => return r
+  | .tau t => test t
+  | .vis i k => .vis i (λ o => test (k o))
+partial_fixpoint
