Test/SimpLang.lean
@@ -1,0 +1,387 @@
+import ITree
+
+open ITree
+open ITree.Effects
+open ITree.Exec
+
+namespace SimpLang
+
+@[ext]
+structure Loc where
+  private mk ::
+  private n : Nat
+deriving Inhabited, Repr, DecidableEq
+
+instance : Ord Loc where
+  compare l₁ l₂ := compare l₁.n l₂.n
+
+instance : Std.TransOrd Loc where
+  eq_swap := by
+    intros l₁ l₂; unfold compare; unfold instOrdLoc; simp;
+    apply Nat.instTransOrd.eq_swap
+  isLE_trans := by
+    intros l₁ l₂ l₃; unfold compare; unfold instOrdLoc; simp;
+    apply Nat.instTransOrd.isLE_trans
+
+instance : Std.LawfulEqOrd Loc where
+  eq_of_compare := by
+    intros l₁ l₂; unfold compare; unfold instOrdLoc; simp;
+    intros h; ext; assumption
+
+inductive Binder where
+  | anon
+  | named (name : String)
+deriving Inhabited, Repr, DecidableEq
+
+inductive BaseLit where
+  | int (n : Int)
+  | loc (l : Loc)
+  | unit
+deriving Inhabited, Repr, DecidableEq
+
+inductive BinOp where
+  | plus
+  | eq
+  | pair
+deriving Inhabited, Repr, DecidableEq
+
+inductive UnOp where
+  | fst
+  | snd
+deriving Inhabited, Repr, DecidableEq
+
+inductive HeapOp where
+  | alloc
+  | load
+  | store
+  | faa
+deriving Inhabited, Repr, DecidableEq
+
+mutual
+  inductive Exp : Type where
+    | val (v : Val)
+    | var (x : String)
+    | rec_ (f x : Binder) (e : Exp)
+    | app (e₁ e₂ : Exp)
+    | binOp (op : BinOp) (e₁ e₂ : Exp)
+    | unOp (op : UnOp) (e : Exp)
+    | if (e₀ e₁ e₂ : Exp)
+    | fork (e : Exp)
+    | heapOp (op : HeapOp) (e₁ : Exp) (e₂ : Exp)
+    | assert (e : Exp)
+  deriving Inhabited, Repr, DecidableEq
+  inductive Val : Type where
+    | lit (l : BaseLit)
+    | rec_ (f x : Binder) (e : Exp)
+    | pair (v₁ v₂ : Val)
+  deriving Inhabited, Repr, DecidableEq
+end
+
+def Exp.isVal : Exp → Bool
+  | .val _ => true
+  | _ => false
+
+instance : Coe Nat Val where
+  coe n := .lit $ .int n
+
+instance : Coe Int Val where
+  coe n := .lit $ .int n
+
+instance : Coe Unit Val where
+  coe _ := .lit $ .unit
+
+instance : Coe Val Exp where
+  coe v := .val v
+
+instance : OfNat Val n where
+  ofNat := .lit $ .int n
+
+def Exp.substStr (x : String) (v : Val) (e : Exp) : Exp :=
+  match e with
+  | .val _ => e
+  | .var x' => if x == x' then .val v else e
+  | .rec_ f x' e => .rec_ f x' $ if .named x != f && .named x != x' then e.substStr x v else e
+  | .app e₁ e₂ => .app (e₁.substStr x v) (e₂.substStr x v)
+  | .binOp op e₁ e₂ => .binOp op (e₁.substStr x v) (e₂.substStr x v)
+  | .unOp op e' => .unOp op (e'.substStr x v)
+  | .if e₀ e₁ e₂ => .if (e₀.substStr x v) (e₁.substStr x v) (e₂.substStr x v)
+  | .fork e => .fork (e.substStr x v)
+  | .heapOp op e₁ e₂ => .heapOp op (e₁.substStr x v) (e₂.substStr x v)
+  | .assert e => .assert (e.substStr x v)
+
+def Exp.subst (x : Binder) (v : Val) (e : Exp) : Exp :=
+  if let .named x := x then Exp.substStr x v e else e
+
+def BaseLit.bool (b : Bool) : BaseLit :=
+  if b then .int 1 else .int 0
+
+def Val.int! [failE -< E] : Val → ITree E Int
+  | lit (.int i) => return i
+  | x => fail s!"{reprStr x} is not Int"
+
+def Val.bool! [failE -< E] (v : Val) : ITree E Bool :=
+  do return (← v.int!) != 0
+
+def Val.loc! [failE -< E] : Val → ITree E Loc
+  | lit (.loc l) => return l
+  | x => fail s!"{reprStr x} is not Loc"
+
+def Val.pair! [failE -< E] : Val → ITree E (Val × Val)
+  | .pair v1 v2 => return (v1, v2)
+  | x => fail s!"{reprStr x} is not Pair"
+
+def Val.rec! [failE -< E] : Val → ITree E (Binder × Binder × Exp)
+  | rec_ f x e => return (f, x, e)
+  | x => fail s!"{reprStr x} is not Rec"
+
+abbrev simpE := concE ⊕ₑ heapE Loc Val ⊕ₑ failE ⊕ₑ demonicE Loc
+def simpEH {GE GR} := concEH (GE:=GE) (GR:=GR) ⊕ₑₕ (heapEH Loc Val ⊕ₛₑₕ failEH ⊕ₛₑₕ demonicEH Loc).toEHandler
+
+instance {GE GR GR'} : EHandlerBind (GE:=GE) (GR:=GR) (GR':=GR')
+  simpEH (failingEH ⊕ₑₕ (heapEH Loc Val ⊕ₛₑₕ failEH ⊕ₛₑₕ demonicEH Loc).toEHandler) := inferInstanceAs (EHandlerBind (concEH ⊕ₑₕ _) _)
+
+def UnOp.denote (op : UnOp) (v : Val) : ITree simpE Val :=
+  match op with
+  | .fst => return (← v.pair!).1
+  | .snd => return (← v.pair!).2
+
+def BinOp.denote (op : BinOp) (v₁ v₂ : Val) : ITree simpE Val :=
+  match op with
+  | .plus => return (← v₁.int!) + (← v₂.int!)
+  | .eq => return .lit (.bool (decide $ v₁ == v₂))
+  | .pair => return .pair v₁ v₂
+
+def HeapOp.denote (op : HeapOp) (v₁ v₂ : Val) : ITree simpE Val :=
+  match op with
+  | .alloc => do
+    let l ← HeapE.alloc v₂
+    return .lit (.loc l)
+  | .load => do load! (← v₁.loc!)
+  | .store => do
+    _ ← store! (← v₁.loc!) v₂
+    return .lit .unit
+  | .faa => do
+    let l ← v₁.loc!
+    let x ← load! l
+    let x' := (← x.int!) + (← v₂.int!)
+    _ ← store! l (x' : Val)
+    return x
+
+def Exp.yieldIfNotVal : Exp → ITree simpE Unit
+  | .val _ => return ()
+  | _ => yield
+
+def Exp.denote (e : Exp) : ITree simpE Val :=
+  let denoteYield e :=
+    if e.isVal then denote e else yieldAfter (denote e)
+  match e with
+  | .val v => return v
+  | .var x => fail s!"Unbound variable {reprStr x}"
+  | .rec_ f x e => return .rec_ f x e
+  | .app e₁ e₂ => do
+    let f ← denoteYield e₁
+    let v ← denoteYield e₂
+    let ⟨f', x', e⟩ ← f.rec!
+    let body := e.subst f' f |>.subst x' v
+    body.yieldIfNotVal
+    denote body
+  | .binOp op e₁ e₂ => do
+    let v₁ ← denoteYield e₁
+    let v₂ ← denoteYield e₂
+    op.denote v₁ v₂
+  | .unOp op e => do
+    let v ← denoteYield e
+    op.denote v
+  | .if e₀ e₁ e₂ => do
+    let c ← denoteYield e₀
+    if ← c.bool! then
+      denoteYield e₁
+    else
+      denoteYield e₂
+  | .fork e => do
+    let _ ← ConcE.fork (denoteYield e >>= λ _ =>return ⟨⟩)
+    return .lit .unit
+  | .heapOp op e₁ e₂ => do
+    let v₁ ← denoteYield e₁
+    let v₂ ← denoteYield e₂
+    op.denote v₁ v₂
+  | .assert e => do
+    let v ← denoteYield e
+    if ← v.bool! then
+      return .lit .unit
+    else
+      fail s!"Assertion failed {reprStr e}"
+partial_fixpoint
+
+/-
+section Notation
+open Lean Elab Elab.Term Parser
+
+abbrev pair := Exp.binOp .pair
+abbrev fst := Exp.unOp .fst
+abbrev snd := Exp.unOp .snd
+abbrev alloc e := Exp.heapOp .alloc (.val $ .lit $ .int 1) e
+abbrev load e := Exp.heapOp .load e (.val $ .lit .unit)
+abbrev store := Exp.heapOp .store
+abbrev faa := Exp.heapOp .faa
+
+instance : Coe Unit Val where
+  coe _ := .lit .unit
+
+declare_syntax_cat simp_binder
+declare_syntax_cat simp_val
+declare_syntax_cat simp_exp
+
+def dollarTerm := leading_parser "$" >> (ident <|> ("(" >> termParser >> ")"))
+
+syntax ("_" <|> ident <|> dollarTerm) : simp_binder
+
+def expandSimpBinder : Syntax → MacroM Term
+  | `(simp_binder| _) => `(Binder.anon)
+  | `(simp_binder| $i:ident) => `(Binder.named $(Syntax.mkStrLit i.raw.getId.toString))
+  | `(simp_binder| $$($t:term)) => return t
+  | s =>
+    -- Lean doesn't allow `(simp_binder| $$$i:ident), so we have to check the syntax manually
+    if s.getKind == `simp_binder.pseudo.antiquot && s.getArgs.size == 4
+        && s[0].getKind == `«$» && s[1].getKind == `null && s[2].getKind == `ident
+        && s[3].getKind == `null
+    then
+      `($(⟨s[2]⟩))
+    else Macro.throwUnsupported
+
+elab "#testBinder " l:simp_binder : command => do
+  let binder ← Command.liftTermElabM $ elabTerm (← liftMacroM $ expandSimpBinder l) (some (.const `HITrees.Examples.SimpLang.Binder []))
+  logInfo m!"{binder}"
+  return
+
+syntax:max "()" : simp_val
+syntax:max "-"? num : simp_val
+syntax:max "(" simp_val ", " simp_val,+ ")" : simp_val
+syntax:10 "λ " simp_binder+ " , " simp_exp:10 : simp_val
+syntax:10 "rec " simp_binder ppSpace simp_binder+ " := " simp_exp:10 : simp_val
+syntax:max dollarTerm : simp_val
+
+/- simp_exp -/
+syntax:max "(" simp_exp ")" : simp_exp
+syntax:max ident : simp_exp -- var
+syntax:max "# " simp_val : simp_exp -- val
+
+syntax:65 simp_exp:66 " + " simp_exp:65 : simp_exp -- plus
+syntax:60 simp_exp:61 " = " simp_exp:60 : simp_exp -- eq
+syntax:max "(" simp_exp ", " simp_exp,+ ")" : simp_exp -- pair
+
+syntax:100 "fst " simp_exp:101 : simp_exp -- fst
+syntax:100 "snd " simp_exp:101: simp_exp -- fst
+
+syntax:max "! " simp_exp:(max-1) : simp_exp -- load
+syntax:max "ref " simp_exp : simp_exp -- alloc
+syntax:15 simp_exp:15 " ← " simp_exp:15 : simp_exp -- store
+syntax:100 "FAA " simp_exp:101 ppSpace simp_exp:101 : simp_exp -- FAA
+
+syntax:9 simp_exp:10 " || " simp_exp:9 : simp_exp -- par
+
+syntax:max "call/cc " "(" "λ " simp_binder ", "  simp_exp:1 ")" : simp_exp -- callcc
+syntax:50 "throw " simp_exp:51 " to " simp_exp:51 : simp_exp -- throw
+
+syntax:100 simp_exp:100 simp_exp:101 : simp_exp -- app
+syntax:10 "if " simp_exp:10 " then " simp_exp:10 " else " simp_exp:10 : simp_exp -- if
+
+syntax:10 "let " simp_binder " := " simp_exp:10 " in " simp_exp:1 : simp_exp -- let
+syntax:5 simp_exp:6 "; " simp_exp:5 : simp_exp -- seq
+syntax:10 "λ " simp_binder+ ", " simp_exp:10 : simp_exp -- lam
+syntax:10 "rec " simp_binder ppSpace simp_binder+ " := " simp_exp:10 : simp_exp -- rec
+
+
+syntax:max "skip" : simp_exp
+syntax:max "assert " simp_exp:max : simp_exp
+syntax:max dollarTerm : simp_exp
+
+mutual
+partial def expandSimpVal : Syntax → MacroM Term
+  | `(simp_val| ()) => `(Val.lit .unit)
+  | `(simp_val| $n:num) => `(Val.lit $ .int $n)
+  | `(simp_val| -$n:num) => `(Val.lit $ .int (Int.neg $n))
+  | `(simp_val| ($x, $y)) => do `(Val.pair $(← expandSimpVal x) $(← expandSimpVal y))
+  | `(simp_val| ($x, $y, $zs,*)) => do
+    let rest ← `(simp_val| ($y, $zs,*))
+    `(Val.pair $(← expandSimpVal x) $(← expandSimpVal rest))
+  | `(simp_val| rec $f:simp_binder $x:simp_binder := $e:simp_exp) => do
+    `(Val.rec_ $(← expandSimpBinder f) $(← expandSimpBinder x) $(← expandSimpExp e))
+  | `(simp_val| rec $f:simp_binder $x:simp_binder $xs:simp_binder* := $e:simp_exp) => do
+    let rest ← `(simp_exp| rec _ $xs* := $e)
+    `(Val.rec_ $(← expandSimpBinder f) $(← expandSimpBinder x) $(← expandSimpExp rest))
+  | `(simp_val| λ $x:simp_binder , $e:simp_exp) => do
+    `(Val.rec_ Binder.anon $(← expandSimpBinder x) $(← expandSimpExp e))
+  | `(simp_val| λ $x:simp_binder $xs:simp_binder* , $e:simp_exp) => do
+    let rest ← `(simp_exp| λ $xs* , $e)
+    `(Val.rec_ Binder.anon $(← expandSimpBinder x) $(← expandSimpExp rest))
+  | `(simp_val| $$($t:term)) => return t
+  | s =>
+    -- Lean doesn't allow `(simp_val| $$$i:ident), so we have to check the syntax manually
+    if s.getKind == `simp_val.pseudo.antiquot && s.getArgs.size == 4
+        && s[0].getKind == `«$» && s[1].getKind == `null && s[2].getKind == `ident
+        && s[3].getKind == `null
+    then
+      `($(⟨s[2]⟩))
+    else Macro.throwUnsupported
+
+partial def expandSimpExp : Syntax → MacroM Term
+  /- parentheses, var, and val -/
+  | `(simp_exp| ($e)) => expandSimpExp e
+  | `(simp_exp| $b:ident) => do `(Exp.var $(Syntax.mkStrLit b.raw.getId.toString))
+  | `(simp_exp| # $v) => do `(Exp.val $(← expandSimpVal v))
+  /- binOp -/
+  | `(simp_exp| $e₁ + $e₂) => do `(Exp.binOp .plus $(← expandSimpExp e₁) $(← expandSimpExp e₂))
+  | `(simp_exp| $e₁ = $e₂) => do `(Exp.binOp .eq $(← expandSimpExp e₁) $(← expandSimpExp e₂))
+  | `(simp_exp| ($x, $y)) => do `(pair $(← expandSimpExp x) $(← expandSimpExp y))
+  | `(simp_exp| ($x, $y, $zs,*)) => do
+    let rest ← `(simp_exp| ($y, $zs,*))
+    `(pair $(← expandSimpExp x) $(← expandSimpExp rest))
+  /- unOp -/
+  | `(simp_exp| fst $e) => do `(Exp.unOp .fst $(← expandSimpExp e))
+  | `(simp_exp| snd $e) => do `(Exp.unOp .snd $(← expandSimpExp e))
+  /- heap -/
+  | `(simp_exp| ! $e) => do `(load $(← expandSimpExp e))
+  | `(simp_exp| ref $e) => do `(alloc $(← expandSimpExp e))
+  | `(simp_exp| $e₁ ← $e₂) => do `(store $(← expandSimpExp e₁) $(← expandSimpExp e₂))
+  | `(simp_exp| FAA $e₁ $e₂) => do `(faa $(← expandSimpExp e₁) $(← expandSimpExp e₂))
+  /- concurrency -/
+  | `(simp_exp| $e₁ || $e₂) => do `(Exp.par $(← expandSimpExp e₁) $(← expandSimpExp e₂))
+  /- call/cc -/
+  | `(simp_exp| call/cc (λ $x, $e)) => do `(Exp.callcc $(← expandSimpBinder x) $(← expandSimpExp e))
+  | `(simp_exp| throw $e₁ to $e₂) => do `(Exp.throw $(← expandSimpExp e₁) $(← expandSimpExp e₂))
+  /- app -/
+  | `(simp_exp| $e₁ $e₂) => do `(Exp.app $(← expandSimpExp e₁) $(← expandSimpExp e₂))
+  /- if -/
+  | `(simp_exp| if $e₁ then $e₂ else $e₃) => do `(Exp.if $(← expandSimpExp e₁) $(← expandSimpExp e₂) $(← expandSimpExp e₃))
+  /- rec, λ, let in, seq -/
+  | `(simp_exp| let $x := $e₁ in $e₂) => do expandSimpExp $ ← `(simp_exp| (λ $x, $e₂) $e₁)
+  | `(simp_exp| $e₁ ; $e₂) => do expandSimpExp $ ← `(simp_exp| (λ _, $e₂) $e₁)
+  | `(simp_exp| rec $f:simp_binder $x:simp_binder := $e:simp_exp) => do
+    `(Exp.rec_ $(← expandSimpBinder f) $(← expandSimpBinder x) $(← expandSimpExp e))
+  | `(simp_exp| rec $f:simp_binder $x:simp_binder $xs:simp_binder* := $e:simp_exp) => do
+    let rest ← `(simp_exp| rec _ $xs* := $e)
+    `(Exp.rec_ $(← expandSimpBinder f) $(← expandSimpBinder x) $(← expandSimpExp rest))
+  | `(simp_exp| λ $x:simp_binder , $e:simp_exp) => do
+    `(Exp.rec_ Binder.anon $(← expandSimpBinder x) $(← expandSimpExp e))
+  | `(simp_exp| λ $x:simp_binder $xs:simp_binder* , $e:simp_exp) => do
+    let rest ← `(simp_exp| λ $xs* , $e)
+    `(Exp.rec_ Binder.anon $(← expandSimpBinder x) $(← expandSimpExp rest))
+  | `(simp_exp| skip) =>
+    `(Exp.app (Exp.val (Val.rec_ Binder.anon Binder.anon (Exp.val (Val.lit BaseLit.unit)))) (Exp.val (Val.lit BaseLit.unit)))
+  | `(simp_exp| assert $e) => do `(Exp.assert $(← expandSimpExp e))
+  | `(simp_exp| $$($t:term)) => return t
+  | s =>
+    -- Lean doesn't allow `(simp_exp| $$$i:ident), so we have to check the syntax manually
+    if s.getKind == `simp_exp.pseudo.antiquot && s.getArgs.size == 4
+        && s[0].getKind == `«$» && s[1].getKind == `null && s[2].getKind == `ident
+        && s[3].getKind == `null
+    then
+      `($(⟨s[2]⟩))
+    else Macro.throwUnsupported
+
+
+end
+
+elab "[SIMP| " e:simp_exp "]" : term => do elabTerm (← liftMacroM $ expandSimpExp e) (some (.const `HITrees.Examples.SimpLang.Exp []))
+-/
